src3.0/Transforms/sas.v
@@ -1116,7 +1116,7 @@ Proof.
 Qed.
 *)
 
-Lemma callExternalFunction__mem_simulation_l2r: forall pinfo sasinfo 
+Axiom callExternalFunction__mem_simulation_l2r: forall pinfo sasinfo 
   TD St1 M1 M2 fid0 gvss0 oresult1 M1' dck tr1 gl tret targs,
   mem_simulation pinfo sasinfo TD St1 M1 M2 ->
   callExternalOrIntrinsics TD gl M1 fid0 tret targs dck gvss0 =
@@ -1126,7 +1126,6 @@ Lemma callExternalFunction__mem_simulation_l2r: forall pinfo sasinfo
       ret (oresult2, tr2, M2') /\
     oresult1 = oresult2 /\ mem_simulation pinfo sasinfo TD St1 M1' M2' /\ 
     tr1 = tr2.
-Admitted. (* excall sim *)
 
 Lemma callExternalFunction__mem_simulation: forall pinfo sasinfo TD St1 M1 M2
   fid0 gvss0 oresult1 M1' oresult2 M2' dck tret targs gl tr1 tr2,
